IL/ILN.v
@@ -114,13 +114,11 @@ Module F.
         destruct (get_dec F' f') as [[[[l' Z] s] ?]|].
         * decide (l = l'); subst.
           decide (length Z = length Y).
-          Start Profiling.
-          case_eq (omap (exp_eval V) Y); intros; try now (right; stuck2).
+          case_eq (omap (exp_eval V) Y); intros; [| right; stuck2].
           left. eexists EvtTau. econstructor. econstructor; eauto.
           orewrite (l' + 0=l'). eauto.
           right; stuck2. rewrite Ldef in H. inv H. get_functional; subst. congruence.
           right; stuck2. rewrite Ldef in H. inv H. get_functional; subst. congruence.
-          Show Profile.
         * right; stuck2. rewrite Ldef in H. inv H. eauto.
       + right. stuck.
     - right. stuck.
@@ -310,11 +308,13 @@ Lemma pos_drop_eq symb (l:lab) x
   -> drop x symb = l::tl (drop x symb).
 Proof.
   general induction symb.
-  unfold pos in H; fold pos in H. cases in H.
-  inv H; inv COND; eauto.
-  destruct x. exfalso. exploit (pos_ge _ _ _ H); eauto. omega.
-  simpl. erewrite IHsymb; eauto.
-  eapply (pos_sub 1); eauto.
+  unfold pos in H; fold pos in H.
+  cases in H; simpl; eauto.
+  - inv COND; eauto.
+  - destruct x.
+    + exfalso. exploit (pos_ge _ _ _ H); eauto. omega.
+    + simpl. erewrite IHsymb; eauto.
+      eapply (pos_sub 1); eauto.
 Qed.
 
 Lemma pos_plus symb (f:lab) n i
